theories/sim/invariant_access.v
@@ -13,23 +13,25 @@ Qed.
 
 Lemma priv_loc_not_public r l t t' :
   priv_loc r l t →
-  (∃ (h: heapletR), r.(rtm) !! t' ≡ Some (to_tagKindR tkPub, h)) →
+  (∃ (h: heapletR), r.(rtm) !! t' ≡ Some (to_tgkR tkPub, h)) →
   t ≠ t'.
 Proof.
   intros [h1 [Eqh1 ?]] [h2 Eqh2] ?. subst t'. move : Eqh2. rewrite Eqh1.
   intros [Eq1 ?]%Some_equiv_inj. by inversion Eq1.
 Qed.
 
-Lemma local_access_eq r l t t' stk n stk' kind σs σt :
+Lemma local_access_eq r l tls t t' stk n stk' kind σs σt :
   σt.(sst) !! l = Some stk →
   access1 stk kind t' σt.(scs) = Some (n, stk') →
   wsat r σs σt →
-  (r.(rlm) !! l : optionR tagR) ≡ Some (to_tagR t) →
+  r.(rlm) !! t ≡ Some (Excl tls) →
+  l ∈ tls →
   t' = Tagged t ∧ stk' = stk.
 Proof.
-  intros Eql Eqstk WSAT Eqt'.
+  intros Eql Eqstk WSAT Eqt' Inl.
   destruct WSAT as (WFS & WFT & VALID & PINV & CINV & SREL & LINV).
-  specialize (LINV _ _ Eqt') as [? [Eqs ?]]. rewrite Eql in Eqs. simplify_eq.
+  specialize (LINV _ _ Eqt') as [? Eqs]. specialize (Eqs _ Inl).
+  rewrite Eql in Eqs. simplify_eq.
   destruct (access1_in_stack _ _ _ _ _ _ Eqstk)
     as [it [?%elem_of_list_singleton [Eqt ?]]].
   subst. split; [done|].
@@ -45,20 +47,20 @@ Lemma priv_loc_UB_access_eq r l kind σs σt t t' stk :
   priv_loc r l t →
   t' = Tagged t.
 Proof.
-  intros Eql ACC WSAT (h & Eqh & [LOC|PRO]).
+  intros Eql ACC WSAT (h & Eqh & Inl & [[tls []]|PRO]).
   { destruct ACC as [[]]. eapply local_access_eq; eauto. }
   destruct WSAT as (WFS & WFT & VALID & PINV & CINV & SREL & LINV).
   specialize (PINV _ _ _ Eqh) as [Lt PINV].
-  destruct PRO as (c & T & Eqc & InT & Inl). have Inl' := Inl.
+  destruct PRO as (c & T & tls & Eqc & EqT & Intls). have Inl' := Inl.
   move : Inl'. rewrite elem_of_dom. intros [sa Eqs].
   move : (proj1 (proj1 VALID) t). rewrite Eqh. intros [_ VALh].
   specialize (VALh l). rewrite Eqs in VALh.
-  apply to_agree_uninj in VALh as [s Eqsa].
-  have Eqss : h !! l ≡ Some (to_agree s) by rewrite Eqsa Eqs.
-  specialize (PINV _ _ Eqss stk Eql).
-  specialize (CINV _ _ Eqc). simpl in CINV. destruct CINV as [Ltc CINV].
-  specialize (CINV _ InT) as [Ltt CIN].
-  specialize (CIN _ _ Eqh _ Inl) as (stk1 & pm1 & Eqstk1 & In1 & NDIS1).
+  apply to_agree_uninj in VALh as [[ss st] Eqsa].
+  have Eqss : h !! l ≡ Some (to_agree (ss, st)) by rewrite Eqsa Eqs.
+  specialize (PINV _ _ _ Eqss stk Eql).
+  specialize (CINV _ _ Eqc) as [Ltc CINV].
+  specialize (CINV _ _ EqT) as [Ltt CINV].
+  specialize (CINV _ Intls) as (stk1 & pm1 & Eqstk1 & In1 & NDIS1).
   rewrite Eqstk1 in Eql. simplify_eq.
   specialize (PINV _ _ In1 NDIS1) as [Eqs1 [? HD]].
 
@@ -72,7 +74,7 @@ Lemma priv_pub_access_UB (r: resUR) l kind σs σt t t' stk :
   wsat r σs σt →
   priv_loc r l t →
   (if t' is (Tagged t2)
-   then ∃ (h: heapletR), r.(rtm) !! t2 ≡ Some (to_tagKindR tkPub, h)
+   then ∃ (h: heapletR), r.(rtm) !! t2 ≡ Some (to_tgkR tkPub, h)
    else True) →
   False.
 Proof.
@@ -83,74 +85,54 @@ Proof.
 Qed.
 
 (** For writing to heaplet *)
-Fixpoint write_heaplet (l: loc) (v: value) (h: heaplet) :=
-  match v with
-  | [] => h
-  | s :: v =>
-      write_heaplet (l +ₗ 1) v (if h !! l then <[l := s]> h else h)
-  end.
-
-Instance write_heaplet_proper (l: loc) (v: value) :
-  Proper ((≡) ==> (≡)) (write_heaplet l v).
+Instance write_hpl_proper (l: loc) v :
+  Proper ((≡) ==> (≡)) (write_hpl l v).
 Proof.
   intros h1 h2 Eq. revert l h1 h2 Eq.
   induction v as [|s v IH]; intros l h1 h2 Eq; simpl; [done|].
-  apply IH. move : (Eq l).
-  destruct (h1 !! l) as [s1|] eqn:Eq1, (h2 !! l) as [s2|] eqn:Eq2; [..|done];
-    rewrite Eq1 Eq2; intros Eql; [by rewrite Eq|by inversion Eql..].
+  apply IH. intros l'.
+  case (decide (l' = l)) => [->|?].
+  - by rewrite 2!lookup_insert.
+  - do 2 (rewrite lookup_insert_ne; [|done]). apply Eq.
 Qed.
 
-Lemma write_heaplet_dom (l: loc) (v: value) h :
-  dom (gset loc) (write_heaplet l v h) ≡ dom (gset loc) h.
+Lemma write_hpl_lookup (l: loc) v (h: heaplet) :
+  (∀ (i: nat) s, (i < length v)%nat →
+    write_hpl l v h !! (l +ₗ i) = Some s →
+    v !! i = Some s) ∧
+  (∀ (l': loc), (∀ (i: nat), (i < length v)%nat → l' ≠ l +ₗ i) →
+    write_hpl l v h !! l' = h !! l').
 Proof.
-  revert l h.
-  induction v as [|s v IH]; intros l h; simpl; [done|].
-  rewrite IH. destruct (h !! l) eqn:Eq; [|done].
-  rewrite dom_map_insert_is_Some //. by eexists.
-Qed.
-
-Lemma write_heaplet_empty l v : write_heaplet l v ∅ ≡ ∅.
-Proof. revert l. induction v as [|?? IH]; [done|]; intros l. apply IH. Qed.
-
-Lemma write_heaplet_lookup (l: loc) (vl: value) (h: heaplet) :
-  (∀ (i: nat) s, (i < length vl)%nat →
-    write_heaplet l vl h !! (l +ₗ i) = Some s →
-    vl !! i = Some s) ∧
-  (∀ (l': loc), (∀ (i: nat), (i < length vl)%nat → l' ≠ l +ₗ i) →
-    write_heaplet l vl h !! l' = h !! l').
-Proof.
-  revert l h. induction vl as [|v vl IH]; move => l h; simpl;
+  revert l h. induction v as [|s v IH]; move => l h; simpl;
     [split; [intros; by lia|done]|].
-  destruct (IH (l +ₗ 1) (if h !! l then <[l:=v]> h else h)) as [IH1 IH2].
+  destruct (IH (l +ₗ 1) (<[l:=s]> h)) as [IH1 IH2].
   split.
-  - intros i s Lt. destruct i as [|i].
-    + rewrite shift_loc_0_nat /=. rewrite IH2; [|].
-      * destruct (h !! l) eqn:Eql; [by rewrite lookup_insert|].
-        rewrite Eql; by inversion 1.
+  - intros i si Lt. destruct i as [|i].
+    + rewrite shift_loc_0_nat /= IH2.
+      * by rewrite lookup_insert.
       * move => ? _.
         rewrite shift_loc_assoc -{1}(shift_loc_0 l) => /shift_loc_inj ?. by lia.
-    + intros Eq. rewrite /= (IH1 _ s) ; [eauto|lia|].
+    + intros Eq. rewrite /= (IH1 _ si) ; [eauto|lia|].
       by rewrite shift_loc_assoc -(Nat2Z.inj_add 1).
   - intros l' Lt. rewrite IH2.
-    + destruct (h !! l) eqn:Eql; [|done].
-      rewrite lookup_insert_ne; [done|].
+    + rewrite lookup_insert_ne; [done|].
       move => ?. subst l'. apply (Lt O); [lia|by rewrite shift_loc_0_nat].
     + move => i Lti. rewrite shift_loc_assoc -(Nat2Z.inj_add 1).
       apply Lt. by lia.
 Qed.
 
-Lemma unique_access_head r σs σ l stk kind n' stk' t s h :
-  σ.(sst) !! l = Some stk →
-  access1 stk kind (Tagged t) σ.(scs) = Some (n', stk') →
-  tmap_inv r σs σ →
-  r.(rtm) !! t ≡ Some (to_tagKindR tkUnique, h) →
-  h !! l ≡ Some $ to_agree s →
+Lemma unique_access_head r σs σt l stk kind n' stk' t ss st h :
+  σt.(sst) !! l = Some stk →
+  access1 stk kind (Tagged t) σt.(scs) = Some (n', stk') →
+  tmap_inv r σs σt →
+  r.(rtm) !! t ≡ Some (to_tgkR tkUnique, h) →
+  h !! l ≡ Some $ to_agree (ss,st) →
   ∃ it, it.(perm) = Unique ∧ it.(tg) = Tagged t ∧ is_stack_head it stk ∧
-    σ.(shp) !! l = Some s.
+    σt.(shp) !! l = Some st ∧ σs.(shp) !! l = Some ss.
 Proof.
   intros Eqstk ACC1 PINV HL Eqs.
   specialize (PINV _ _ _ HL) as [? PINV].
-  specialize (PINV _ _ Eqs _ Eqstk).
+  specialize (PINV _ _ _ Eqs _ Eqstk).
   destruct (access1_in_stack _ _ _ _ _ _ ACC1) as (it & Init & Eqti & NDIS).
   destruct (PINV it.(perm) it.(protector)) as [Eqss [? HD]]; [|done|].
   { rewrite -Eqti. by destruct it. }
